# 2020732014 조현준 과제3  
---
# P3.1  
![image](https://github.com/user-attachments/assets/ea9d86d8-e471-4843-994a-e637c0550b16)  

$M \frac{d^2 y(t)}{dt^2} = F(t) - b \frac{dy(t)}{dt} - k y(t)$  

$x_1(t) = y(t), \quad x_2(t) = \frac{dy(t)}{dt}$ 라고 가정  

$M \cdot \dot{x_2}(t) = F(t) - b x_2(t) - k x_1(t)$  

$\dot{x_2}(t) = - \frac{k}{M} x_1(t) - \frac{b}{M} x_2(t) + \frac{1}{M} F(t)$  

$$ \dot{x}(t) = \begin{vmatrix} 0 && 1 \\
-\frac{k}{M} && -\frac{b}{M} \end{vmatrix} x(t) + \begin{vmatrix} 0 \\
\frac{1}{M} \end{vmatrix}F(t) $$

$$y(t) = \begin{vmatrix} 1 && 0 \end{vmatrix}$$
  
---
# P3.3  
![image](https://github.com/user-attachments/assets/6d153b20-e798-47f4-8e2f-63859b4dc88a)  
$x_1(t) = i_L(t), \quad x_2(t) = v_C(t)$

$\text{KCL:} \quad{i_L}(t) = \frac{v_2(t) - v_C(t)}{R} - C \frac{dV_C(t)}{dt}$

$x_1(t) = \frac{v_2(t) - x_2(t)}{R} - C \frac{dx_2(t)}{dt}$

$\frac{dx_2(t)}{dt} = -\frac{1}{C} x_1(t) + \frac{v_2(t) - x_2(t)}{RC}$

$\frac{dx_2(t)}{dt} = -\frac{1}{C} x_1(t) - \frac{x_2(t)}{RC} + \frac{v_2(t)}{RC}$

$\text{KVL:} \quad -v_1(t) + L \frac{di_L(t)}{dt} - v_C(t) + v_2(t) = 0$

$L \frac{di_L(t)}{dt} = v_1(t) - v_2(t) + v_C(t)$

$\frac{dx_1(t)}{dt} = \frac{v_1(t)}{L} - \frac{v_2(t)}{L} + \frac{x_2(t)}{L}$

$$\dot{x}(t) = \begin{bmatrix} 0 & \frac{1}{L} \\
-\frac{1}{C} & -\frac{1}{RC} \end{bmatrix} \mathbf{x}(t) + \begin{bmatrix} \frac{1}{L} && -\frac{1}{L} \\
0 && \frac{1}{RC} \end{bmatrix} V(t)$$

---
# P3.5  
![image](https://github.com/user-attachments/assets/ea74644d-7a19-46fb-ae75-71cbaeda807d)  
$G(s) = \frac{s + 2}{s + 8} \cdot \frac{1}{s - 3} \cdot \frac{1}{s} = \frac{s + 2}{s(s + 8)(s - 3)}$

$T(s) = \frac{Y(s)}{R(s)}$

$Y(s) = G(s) \left( R(s) - Y(s) \right)$

$Y(s) + G(s) Y(s) = G(s) R(s)$

$Y(s) ( G(s) + 1 ) = G(s) R(s)$

$\therefore T(s) = \frac{Y(s)}{R(s)} = \frac{G(s)}{G(s) + 1} = \frac{\frac{s + 2}{s(s + 8)(s - 3)}}{\frac{s + 2}{s(s + 8)(s - 3)} + 1}$

$= \frac{s + 2}{s(s + 8)(s - 3)} \Bigg/ \frac{(s + 2) + s(s + 8)(s - 3)}{s(s + 8)(s - 3)}$

$= \frac{s + 2}{(s + 2) + s(s + 8)(s - 3)} = \frac{s + 2}{s^3 + 5s^2 - 23s + 2}$

$T(s) = \frac{Y(s)}{R(s)} = \frac{s + 2}{s^3 + 5s^2 - 23s + 2} \cdot \frac{Z(s)}{Z(s)}$

$Y(s) = (s + 2) \cdot Z(s)$

$R(s) = (s^3 + 5s^2 - 23s + 2) \cdot Z(s)$

$\mathcal{L}^{-1}$

$\dddot{z}(t) + 5 \ddot{z}(t) - 23 \dot{z}(t) + 2 z(t) = r(t)$

$\ddddot{z}(t) = -5 \ddot{z}(t) + 23 \dot{z}(t) - 2z(t) + r(t)$

$$\begin{pmatrix} x_1(t) \\
x_2(t) \\
x_3(t) \end{pmatrix} = \begin{pmatrix} z(t) \\
\dot{x_1}(t) \\
\dot{x_2}(t) \end{pmatrix} = \begin{pmatrix} z(t) \\
\dot{z}(t) \\
\ddot{z}(t) \end{pmatrix}$$

$$\dot{x}(t) = \begin{pmatrix} 0 & 1 & 0 \\
0 & 0 & 1 \\
-2 & 23 & -5 \end{pmatrix} x(t) + \begin{pmatrix} 0 \\
0 \\
1 \end{pmatrix} r(t)$$

$$y(t) = \begin{pmatrix} 2 & 1 & 0 \end{pmatrix} x(t)$$

---
# P3.12  
![image](https://github.com/user-attachments/assets/b707d9d0-0888-4f3d-9246-f1c3bc8b94fa)  
a) $\frac{Y(s)}{R(s)} = \frac{8(s+5)}{s^3 + 12s^2 + 44s + 48} \cdot \frac{Z(s)}{Z(s)}$

$Y(s) = 8(s + 5) \cdot Z(s)$

$R(s) = (s^3 + 12s^2 + 44s + 48) \cdot Z(s)$

$\mathcal{L}^{-1}$ $\quad y(t) = 40z(t) + 8 \dot{z}(t)$

$r(t) = \dddot{z}(t) + 48z(t) + 44 \dot{z}(t) + 12 \ddot{z}(t)$

$$\dot{x}(t) = \begin{pmatrix} 0 & 1 & 0 \\
0 & 0 & 1 \\
-44 & -44 & -12 \end{pmatrix} x(t) + \begin{pmatrix} 0 \\
0 \\
1 \end{pmatrix} r(t)$$

$$y(t) = \begin{pmatrix} 40 & 8 & 0 \end{pmatrix} x(t)$$

$\Phi(t) = \mathcal{L}^{-1} \left( \Phi(s) \right) = \mathcal{L}^{-1} \left( (sI - A)^{-1} \right)$

---
# P3.17  
![image](https://github.com/user-attachments/assets/14f0a513-9986-41f2-974a-796b9ca3a51f)  

$\dot{x}(t) = A x(t) + B u(t)$

$y(t) = C x(t) + D u(t)$

$\mathcal{L}$ 변환

$s X(s) = A X(s) + B U(s) \quad \Rightarrow \quad X(s)(s I - A) = B U(s), \quad X(s) = (s I - A)^{-1} B U(s)$

$Y(s) = C X(s) + D U(s) \quad \Rightarrow \quad Y(s) = C (s I - A)^{-1} B U(s) + D U(s)$

$\frac{Y(s)}{U(s)} = C (s I - A)^{-1} B + D$

$\frac{Y(s)}{U(s)} = \frac{4(s - 3)}{s^3 - 14s^2 + 37s + 20}$

